Make progress on bvl_inline proof

compiler/backend/bvl_inlineScript.sml
@@ -5,43 +5,44 @@ val _ = new_theory "bvl_inline";
 (* A function that inlines a function body *)
 
 val inline_def = tDefine "inline" `
-  (inline n code arity [] = []) /\
-  (inline n code arity (x::y::xs) =
-     HD (inline n code arity [x]) :: inline n code arity (y::xs)) /\
-  (inline n code arity [Var v] = [Var v]) /\
-  (inline n code arity [If x1 x2 x3] =
-     [If (HD (inline n code arity [x1]))
-         (HD (inline n code arity [x2]))
-         (HD (inline n code arity [x3]))]) /\
-  (inline n code arity [Let xs x2] =
-     [Let (inline n code arity xs)
-           (HD (inline n code arity [x2]))]) /\
-  (inline n code arity [Raise x1] =
-     [Raise (HD (inline n code arity [x1]))]) /\
-  (inline n code arity [Handle x1 x2] =
-     [Handle (HD (inline n code arity [x1]))
-              (HD (inline n code arity [x2]))]) /\
-  (inline n code arity [Op op xs] =
-     [Op op (inline n code arity xs)]) /\
-  (inline n code arity [Tick x] =
-     [Tick (HD (inline n code arity [x]))]) /\
-  (inline n code arity [Call ticks dest xs] =
-     if (dest = SOME n) /\ (LENGTH xs = arity)
-     then [Let (inline n code arity xs) (mk_tick (SUC ticks) code)]
-     else [Call ticks dest (inline n code arity xs)])`
-  (WF_REL_TAC `measure (exp1_size o SND o SND o SND)`);
+  (inline cs [] = []) /\
+  (inline cs (x::y::xs) =
+     HD (inline cs [x]) :: inline cs (y::xs)) /\
+  (inline cs [Var v] = [Var v]) /\
+  (inline cs [If x1 x2 x3] =
+     [If (HD (inline cs [x1]))
+         (HD (inline cs [x2]))
+         (HD (inline cs [x3]))]) /\
+  (inline cs [Let xs x2] =
+     [Let (inline cs xs)
+           (HD (inline cs [x2]))]) /\
+  (inline cs [Raise x1] =
+     [Raise (HD (inline cs [x1]))]) /\
+  (inline cs [Handle x1 x2] =
+     [Handle (HD (inline cs [x1]))
+              (HD (inline cs [x2]))]) /\
+  (inline cs [Op op xs] =
+     [Op op (inline cs xs)]) /\
+  (inline cs [Tick x] =
+     [Tick (HD (inline cs [x]))]) /\
+  (inline cs [Call ticks dest xs] =
+     case dest of NONE => [Call ticks dest (inline cs xs)] | SOME n =>
+     case lookup n cs of
+     | NONE => [Call ticks dest (inline cs xs)]
+     | SOME (arity,code) => [Let (inline cs xs) (mk_tick (SUC ticks) code)])`
+  (WF_REL_TAC `measure (exp1_size o SND)`);
 
 val inline_ind = theorem"inline_ind";
 
 val LENGTH_inline = store_thm("LENGTH_inline",
-  ``!n code arity xs. LENGTH (inline n code arity xs) = LENGTH xs``,
+  ``!cs xs. LENGTH (inline cs xs) = LENGTH xs``,
   recInduct inline_ind \\ REPEAT STRIP_TAC
-  \\ SIMP_TAC std_ss [Once inline_def,LET_DEF] \\ SRW_TAC [] []);
+  \\ fs [Once inline_def,LET_DEF] \\ rw [] \\ every_case_tac \\ fs []);
 
-val HD_inline = store_thm("HD_inline",
-  ``[HD (inline n code arity [x])] = inline n code arity [x]``,
-  `LENGTH (inline n code arity [x]) = LENGTH [x]` by SRW_TAC [] [LENGTH_inline]
-  \\ Cases_on `inline n code arity [x]` \\ FULL_SIMP_TAC std_ss [LENGTH]
+val HD_inline = store_thm("HD_inline[simp]",
+  ``[HD (inline cs [x])] = inline cs [x]``,
+  `LENGTH (inline cs [x]) = LENGTH [x]` by SRW_TAC [] [LENGTH_inline]
+  \\ Cases_on `inline cs [x]` \\ FULL_SIMP_TAC std_ss [LENGTH]
   \\ Cases_on `t` \\ FULL_SIMP_TAC std_ss [LENGTH,HD] \\ `F` by DECIDE_TAC);
 
 val _ = export_theory();
